unified the read and write ixplens perms into a single permission with a read/write modality

src/LensPerms.v
@@ -35,14 +35,17 @@ Section PLensPerms.
    *** Read and write permissions
    ***)
 
-  (* The permission to write to an ixplens, assuming it already has a value that
-  satisfies a given precondition *)
-  Program Definition ixplens_write_perm_pre ix (pre : Elem -> Prop) : @perm St :=
+  (* A value indicating whether an ixplens permission is a read or write *)
+  Variant RWModality := Write | Read.
+
+  (* The permission to read from or write to an ixplens, assuming it already has
+  a value that satisfies a given precondition *)
+  Program Definition ixplens_perm_pre rw ix (pre : Elem -> Prop) : @perm St :=
     {|
       pre x := exists elem, iget ix x = Some elem /\ pre elem;
       rely x y := iget ix x <> None -> iget ix x = iget ix y;
       guar x y := x = y \/
-                    iget ix x <> None /\ exists elem, y = iput ix x elem;
+                    rw = Write /\ iget ix x <> None /\ exists elem, y = iput ix x elem;
       inv x := True
     |}.
   Next Obligation.
@@ -54,9 +57,9 @@ Section PLensPerms.
     constructor; repeat intro.
     - left; reflexivity.
     - destruct H; [ subst; assumption | ].
-      destruct H0 as [? | [? [elem2 ?]]]; [ subst; right; eassumption | ].
-      destruct H as [? [elem1 ?]]. right; subst.
-      split; [ assumption | ].
+      destruct H0 as [? | [? [? [elem2 ?]]]]; [ subst; right; eassumption | ].
+      destruct H as [? [? [elem1 ?]]]. right; subst.
+      repeat (split; [ assumption | ]).
       exists elem2. apply iPutPut; assumption.
   Qed.
   Next Obligation.
@@ -64,97 +67,50 @@ Section PLensPerms.
     eexists; split; eassumption.
   Qed.
 
-  (* Permission to write to an ixplens that already equals a specific value *)
-  Definition ixplens_write_perm_eq ix elem :=
-    ixplens_write_perm_pre ix (eq elem).
+  (* Permission to an ixplens that already equals a specific value *)
+  Definition ixplens_perm_eq rw ix elem :=
+    ixplens_perm_pre rw ix (eq elem).
 
-  (* Permission to write to an ixplens that could be any value *)
-  Definition ixplens_write_perm_any ix :=
-    ixplens_write_perm_pre ix (fun _ => True).
+  (* Permission to an ixplens that could be any value *)
+  Definition ixplens_perm_any rw ix :=
+    ixplens_perm_pre rw ix (fun _ => True).
 
   (* Write permissions are monotonic in their precondition *)
-  Lemma monotone_ixplens_write_perm ix (pre1 pre2 : Elem -> Prop) :
+  Lemma monotone_ixplens_perm rw ix (pre1 pre2 : Elem -> Prop) :
     (forall elem, pre1 elem -> pre2 elem) ->
-    ixplens_write_perm_pre ix pre2 <= ixplens_write_perm_pre ix pre1.
+    ixplens_perm_pre rw ix pre2 <= ixplens_perm_pre rw ix pre1.
   Proof.
     constructor; intros; try assumption.
     destruct H1 as [elem [? ?]]. eexists; split; [ | apply H ]; eassumption.
   Qed.
-
-
-  (* The permission to read from an ixplens, assuming it already has a value *)
-  Program Definition ixplens_read_perm_pre ix (pre : Elem -> Prop) : @perm St :=
-    {|
-      pre x := exists elem, iget ix x = Some elem /\ pre elem;
-      rely x y := iget ix x <> None -> iget ix x = iget ix y;
-      guar x y := x = y;
-      inv x := True
-    |}.
-  Next Obligation.
-    constructor; repeat intro.
-    - reflexivity.
-    - rewrite <- (H H1) in H0. apply H0; assumption.
-  Qed.
-  Next Obligation.
-    rewrite <- H; [ | eapply Some_not_None; eassumption ].
-    eexists; split; eassumption.
-  Qed.
-
-  (* Permission to read from an ixplens that already equals a specific value *)
-  Definition ixplens_read_perm_eq ix elem :=
-    ixplens_read_perm_pre ix (eq elem).
-
-  (* Permission to read from an ixplens that could be any value *)
-  Definition ixplens_read_perm_any ix :=
-    ixplens_read_perm_pre ix (fun _ => True).
-
-  (* Read permissions are monotonic in their precondition *)
-  Lemma monotone_ixplens_read_perm ix (pre1 pre2 : Elem -> Prop) :
-    (forall elem, pre1 elem -> pre2 elem) ->
-    ixplens_read_perm_pre ix pre2 <= ixplens_read_perm_pre ix pre1.
-  Proof.
-    constructor; intros; try assumption.
-    destruct H1 as [elem [? ?]]. eexists; split; [ | apply H ]; eassumption.
-  Qed.
-
 
   (* A write permission is greater than a read permission *)
   Lemma lte_read_write ix pre :
-    ixplens_read_perm_pre ix pre <= ixplens_write_perm_pre ix pre.
+    ixplens_perm_pre Read ix pre <= ixplens_perm_pre Write ix pre.
   Proof.
     constructor; intros.
     - apply H0.
     - apply H0.
-    - inversion H0; reflexivity.
+    - destruct H0 as [? | [? [? [? ?]]]]; subst; [ reflexivity | inversion H0 ].
     - apply I.
   Qed.
 
   (* Read permissions are always separate *)
   Lemma ixplens_read_read_sep ix1 pre1 ix2 pre2 :
-    ixplens_read_perm_pre ix1 pre1 ⊥ ixplens_read_perm_pre ix2 pre2.
+    ixplens_perm_pre Read ix1 pre1 ⊥ ixplens_perm_pre Read ix2 pre2.
   Proof.
-    constructor; intros; inversion H1; reflexivity.
+    constructor; intros;
+      (destruct H1 as [? | [? ?]]; subst; [ reflexivity | inversion H1 ]).
   Qed.
 
-  (* Write permissions with different indices are separate *)
-  Lemma ixplens_write_write_sep ix1 pre1 ix2 pre2 :
-    ix1 <> ix2 -> ixplens_write_perm_pre ix1 pre1 ⊥ ixplens_write_perm_pre ix2 pre2.
+  (* Read/Write permissions with different indices are separate *)
+  Lemma ixplens_uneq_ixs_sep rw1 ix1 pre1 rw2 ix2 pre2 :
+    ix1 <> ix2 -> ixplens_perm_pre rw1 ix1 pre1 ⊥ ixplens_perm_pre rw2 ix2 pre2.
   Proof.
     constructor; intros.
-    - destruct H2 as [? | [? [elem ?]]]; subst; [ reflexivity | ].
+    - destruct H2 as [? | [? [? [elem ?]]]]; subst; [ reflexivity | ].
       intro; symmetry; apply iGetPut_neq; assumption.
-    - destruct H2 as [? | [? [elem ?]]]; subst; [ reflexivity | ].
-      intro; symmetry; apply iGetPut_neq; try assumption.
-      intro; subst; apply H; reflexivity.
-  Qed.
-
-  (* Write and read with different indices are separate *)
-  Lemma ixplens_write_read_sep ix1 pre1 ix2 pre2 :
-    ix1 <> ix2 -> ixplens_write_perm_pre ix1 pre1 ⊥ ixplens_read_perm_pre ix2 pre2.
-  Proof.
-    constructor; intros.
-    - inversion H2; reflexivity.
-    - destruct H2 as [? | [? [elem ?]]]; subst; [ reflexivity | ].
+    - destruct H2 as [? | [? [? [elem ?]]]]; subst; [ reflexivity | ].
       intro; symmetry; apply iGetPut_neq; try assumption.
       intro; subst; apply H; reflexivity.
   Qed.
@@ -164,56 +120,19 @@ Section PLensPerms.
    *** Read and write permission sets
    ***)
 
-  (* A value indicating whether an ixplens permission is a read or write *)
-  Variant RWModality := Write | Read.
-
-  (* A read or write permission whose contents equal a value *)
-  Definition ixplens_perm_eq rw ix elem :=
-    match rw with
-    | Write => ixplens_write_perm_eq ix elem
-    | Read => ixplens_read_perm_eq ix elem
-    end.
-
   (* Dependent write permissions are permissions to write to ix along with
   permission P to the value that is currently stored at ix *)
-  Definition ixplens_write_dep ix (P : Elem -> Perms) : Perms :=
-    meet_Perms
-      (fun R => exists elem,
-           R = singleton_Perms (ixplens_write_perm_eq ix elem) * (P elem)).
-
-  (* Dependent read permissions are permissions to read from ix along with
-  permission P to the value that is currently stored at ix *)
-  Definition ixplens_read_dep ix (P : Elem -> Perms) : Perms :=
-    meet_Perms
-      (fun R => exists elem,
-           R = singleton_Perms (ixplens_read_perm_eq ix elem) * (P elem)).
-
-  (* An ixplens permission that is either write or read *)
-  Definition ixplens_dep rw ix P :=
-    match rw with
-    | Write => ixplens_write_dep ix P
-    | Read => ixplens_read_dep ix P
-    end.
-
-  (* An alternate definition of ixplens_dep as a meet *)
-  Definition ixplens_dep_alt rw ix P :=
+  Definition ixplens_dep rw ix (P : Elem -> Perms) : Perms :=
     meet_Perms
       (fun R => exists elem,
            R = singleton_Perms (ixplens_perm_eq rw ix elem) * (P elem)).
-
-  (* The two definitions of ixplens_dep are equal *)
-  Lemma ixplens_dep_alt_eq rw ix P :
-    ixplens_dep rw ix P ≡ ixplens_dep_alt rw ix P.
-  Proof.
-    destruct rw; reflexivity.
-  Qed.
 
   (* The entailment rule for writing to a dependent write permission, which says
   that if you have write_dep perms to ix then putting elem to ix results in a
   write_dep permission whose contents equal elem *)
   Lemma ixplens_write_ent ix P elem :
-    rewind (fun x => iput ix x elem) (ixplens_write_dep ix P)
-      ⊨ ixplens_write_dep ix (fun e => prop_Perms (e = elem)).
+    rewind (fun x => iput ix x elem) (ixplens_dep Write ix P)
+      ⊨ ixplens_dep Write ix (fun e => prop_Perms (e = elem)).
   Proof.
     apply bigger_Perms_entails. repeat intro.
     simpl in H; destruct_ex_conjs H; subst.
@@ -226,15 +145,15 @@ Section PLensPerms.
     - simpl in H0. destruct_ex_conjs H0; subst.
       exists elem. split; [ | reflexivity ].
       transitivity (iget ix (iput ix x3 elem)); [ | apply iGetPut_eq ].
-      symmetry. eapply (rely_inc (ixplens_write_perm_eq ix x2) x0); try assumption.
+      symmetry. eapply (rely_inc (ixplens_perm_eq Write ix x2) x0); try assumption.
       + rewrite <- lte_l_sep_conj_Perms in H3. apply H3.
       + rewrite iGetPut_eq. eapply Some_not_None; reflexivity.
     - rewrite <- lte_l_sep_conj_Perms in H3.
-      apply (rely_inc (ixplens_write_perm_eq ix x2) x0); assumption.
+      apply (rely_inc (ixplens_perm_eq Write ix x2) x0); assumption.
     - rewrite <- lte_l_sep_conj_Perms in H3.
-      apply (guar_inc (ixplens_write_perm_eq ix x2) x0); assumption.
+      apply (guar_inc (ixplens_perm_eq Write ix x2) x0); assumption.
     - rewrite <- lte_l_sep_conj_Perms in H3.
-      apply (inv_inc (ixplens_write_perm_eq ix x2) x0); assumption.
+      apply (inv_inc (ixplens_perm_eq Write ix x2) x0); assumption.
   Qed.
 
 
@@ -248,10 +167,9 @@ Section PLensPerms.
     add_poss_pre pred (ixplens_dep rw ix P)
       ⊨ ixplens_dep rw ix (fun e => prop_Perms (e = elem)) * P elem.
   Proof.
-    intro. repeat rewrite ixplens_dep_alt_eq.
-    apply add_poss_pre_meet_ent. intros. destruct H0; subst.
+    intro. apply add_poss_pre_meet_ent. intros. destruct H0; subst.
     etransitivity; [ apply add_pre_ent_P | ].
-    unfold ixplens_dep_alt. rewrite sep_conj_Perms_meet_commute.
+    unfold ixplens_dep. rewrite sep_conj_Perms_meet_commute.
     eapply ent_meet_Perms.
     eexists; split; [ eexists; split; [ reflexivity | exists elem; reflexivity ] | ].
     assert (x0 = elem).
@@ -304,11 +222,11 @@ Section PLensPerms.
     - apply I.
   Qed.
 
-  (* A multi-write permission is always separate from a write permission to an
-  index not in the set of the multi-write *)
-  Lemma ixplens_write_multi_write_sep ix pre ixs :
+  (* A multi-write permission is always separate from a read/write permission to
+     an index not in the set of the multi-write *)
+  Lemma ixplens_write_multi_write_sep rw ix pre ixs :
     ~ ixs ix -> self_contained_ixs ixs ->
-    ixplens_write_perm_pre ix pre ⊥ ixplens_multi_write_perm ixs.
+    ixplens_perm_pre rw ix pre ⊥ ixplens_multi_write_perm ixs.
   Proof.
     intros not_in self_c; constructor; repeat intro.
     - clear H H0.
@@ -323,7 +241,7 @@ Section PLensPerms.
       + destruct (IHclos_refl_trans1 H2).
         destruct (IHclos_refl_trans2 H0).
         split; [ etransitivity | ]; eassumption.
-    - destruct H1 as [? | [? [elem ?]]]; subst; [ reflexivity | ].
+    - destruct H1 as [? | [? [? [elem ?]]]]; subst; [ reflexivity | ].
       symmetry; apply self_c; assumption.
   Qed.
 
@@ -331,13 +249,13 @@ Section PLensPerms.
   Lemma ixplens_multi_write_split_write_step ixs ix pre :
     self_contained_ixs ixs ->
     sep_step (ixplens_multi_write_perm (eq ix \1/ ixs))
-      (ixplens_write_perm_pre ix pre ** ixplens_multi_write_perm ixs).
+      (ixplens_perm_pre Write ix pre ** ixplens_multi_write_perm ixs).
   Proof.
     intros; apply sep_step_rg; intros.
     - apply I.
     - clear H0. induction H1; [ | etransitivity; eassumption ].
       destruct H0.
-      + destruct H0 as [? | [? [elem ?]]]; subst; [ reflexivity | ].
+      + destruct H0 as [? | [? [? [elem ?]]]]; subst; [ reflexivity | ].
         apply rt_step; exists ix; exists elem.
         split; [ left | ]; reflexivity.
       + induction H0.
@@ -359,7 +277,7 @@ Section PLensPerms.
     rewind_perm (fun x => iput ix x elem)
       (ixplens_multi_write_perm (eq ix \1/ ixs))
       (ixplens_multi_write_perm (eq ix \1/ ixs))
-      ⊢ ixplens_write_perm_eq ix elem ** ixplens_multi_write_perm ixs.
+      ⊢ ixplens_perm_eq Write ix elem ** ixplens_multi_write_perm ixs.
   Proof.
     intros; apply sep_step_entails_perm.
     - etransitivity; [ apply set_pre_sep_step
